Object.dfy
@@ -1,5 +1,5 @@
 include "Library.dfy"
-  //include "Mode.dfy"
+//include "Mode.dfy"
 include "Ownership.dfy" //comes in via Mode anyway..
 
 //TODOS when valid - precondition on comoputeWOwnerForClone - see JDVANCE
