Ownership-Recursive.dfy
@@ -1,6 +1,6 @@
 include "Klon.dfy"
 include "Set-Lemmata.dfy"
-include "BROWNE.dfy"
+//include "BROWNE.dfy"
 
 //first chunk is "recursice ownership"
 //rest is - likely not needed?
